small commit

src/ConcreteBigraphs.v
@@ -16,7 +16,7 @@ Set Printing All.
 (** This module implements bigraphs and basic operations on bigraphs *)
 Module Bigraphs.
 
-Variable Kappa:Type.
+Parameter Kappa:Type.
 Variable Arity:Kappa-> nat.
 
 (** * Definition of a bigraph
@@ -112,7 +112,7 @@ Record bigraph  (site: FinDecType)
   { 
     node : FinDecType ;
     edge : FinDecType ;
-    control : (type node) -> Bigraphs.Kappa ;
+    control : (type node) -> Kappa ;
     parent : (type node) + (type site) -> (type node) + (type root) ; 
     link : (type innername) + Port control -> (type outername) + (type edge); 
     ap : FiniteParent parent ;
@@ -378,15 +378,10 @@ Definition bigraph_juxtaposition {s1 i1 r1 o1 s2 i2 r2 o2 : FinDecType}
 
 Notation "b1 || b2" := (bigraph_juxtaposition b1 b2) (at level 50, left associativity).
 
-(** * Disjoint juxtaposition
-  This section deals with the operation of disjoint juxtaposition. This is the act
-  of putting two bigraphs with disjoint interfaces "next" to one another. 
-  After the definition, we prove associativity and commutativity of dis_juxtaposition *)
-Section DisjointJuxtaposition.
-Definition bigraph_empty : bigraph findec_void findec_void findec_void findec_void.
+Definition bigraph_empty : bigraph voidfd voidfd voidfd voidfd.
   Proof.
-  apply (Big findec_void findec_void findec_void findec_void
-            findec_void findec_void
+  apply (Big voidfd voidfd voidfd voidfd
+            voidfd voidfd
             (@void_univ_embedding _)
             (choice void_univ_embedding void_univ_embedding)
             (choice void_univ_embedding (void_univ_embedding <o> (bij_port_void (@void_univ_embedding _))))).
@@ -395,6 +390,12 @@ Definition bigraph_empty : bigraph findec_void findec_void findec_void findec_vo
   Defined.
 
 Notation "∅" := bigraph_empty.
+
+(** * Disjoint juxtaposition
+  This section deals with the operation of disjoint juxtaposition. This is the act
+  of putting two bigraphs with disjoint interfaces "next" to one another. 
+  After the definition, we prove associativity and commutativity of dis_juxtaposition *)
+Section DisjointJuxtaposition.
 Lemma arity_juxt_left_neutral : forall {s i r o} (b : bigraph s i r o) n, 
         Arity (get_control (∅ || b) n) = Arity (get_control b (bij_void_sum_neutral n)).
   Proof.
@@ -405,10 +406,10 @@ Lemma arity_juxt_left_neutral : forall {s i r o} (b : bigraph s i r o) n,
   Qed.
 
 Theorem bigraph_juxt_left_neutral : forall {s i r o} (b : bigraph s i r o), 
-  bigraph_equality (bigraph_empty || b) b.
+  bigraph_equality (∅ || b) b.
   Proof.
   intros s i r o b.
-  apply (BigEq _ _ _ _ _ _ _ _ (bigraph_empty || b) b
+  apply (BigEq _ _ _ _ _ _ _ _ (∅ || b) b
           bij_void_sum_neutral
           bij_void_sum_neutral
           bij_void_sum_neutral
@@ -695,7 +696,7 @@ Add Parametric Morphism : bigraph_packed_juxtaposition with
   Qed.
 
 Theorem bigraph_packed_juxt_left_neutral : forall {s i r o} (b : bigraph s i r o), 
-  bigraph_packed_equality (bigraph_packed_juxtaposition bigraph_empty b) b.
+  bigraph_packed_equality (bigraph_packed_juxtaposition ∅ b) b.
   Proof.
   unfold bigraph_packed_equality, bigraph_packed_juxtaposition.
   intros.
@@ -718,7 +719,7 @@ Theorem bigraph_packed_juxt_assoc : forall {s1 i1 r1 o1 s2 i2 r2 o2 s3 i3 r3 o3}
   apply bigraph_juxt_assoc.
   Qed.
 
-Lemma bigraph_juxt_right_neutral : forall {s i r o} (b : bigraph s i r o), bigraph_packed_equality (bigraph_packed_juxtaposition b bigraph_empty) b.
+Lemma bigraph_juxt_right_neutral : forall {s i r o} (b : bigraph s i r o), bigraph_packed_equality (bigraph_packed_juxtaposition b ∅) b.
   Proof.
   intros.
   rewrite bigraph_packed_juxt_comm.
@@ -754,8 +755,8 @@ Section CompositionBigraphs.
 Definition bigraph_identity {s i}: bigraph s i s i.
   Proof.
   apply (Big s i s i
-          findec_void 
-          findec_void
+          voidfd 
+          voidfd
           (@void_univ_embedding _)
           id).
   - intros [inner | p].
@@ -1180,8 +1181,8 @@ Theorem bigraph_comp_juxt_dist : forall {s1 i1 r1 o1 s2 i2 r2 o2 s3 i3 s4 i4}
 Section NestingBig.
 
 Definition rm_void_parent {s1 r1 node0: FinDecType} 
-  (p : type node0 + type (findec_sum findec_void s1) ->
-    type node0 + type (findec_sum findec_void r1)) : 
+  (p : type node0 + type (findec_sum voidfd s1) ->
+    type node0 + type (findec_sum voidfd r1)) : 
     type node0 + type s1 -> type node0 + type r1.
   Proof. intros [n|s].
     - destruct (p (inl n)) eqn:Epn.
@@ -1191,7 +1192,7 @@ Definition rm_void_parent {s1 r1 node0: FinDecType}
     + left. exact t.
     + right. destruct t. destruct t. exact t. Defined.
 
-Definition rm_void_sumtype {r1 : FinDecType} (x:type (findec_sum findec_void r1)) : type r1 := 
+Definition rm_void_sumtype {r1 : FinDecType} (x:type (findec_sum voidfd r1)) : type r1 := 
   match x with
     | inl t =>
         match t return (type r1) with
@@ -1199,11 +1200,11 @@ Definition rm_void_sumtype {r1 : FinDecType} (x:type (findec_sum findec_void r1)
     | inr t => t end.
   (* destruct x. destruct t. exact t. Defined. *)
 
-Definition rm_void_sumtype' {r1 : FinDecType} (x:type (findec_sum findec_void r1)) : type r1.
+Definition rm_void_sumtype' {r1 : FinDecType} (x:type (findec_sum voidfd r1)) : type r1.
   Proof.
   destruct x. destruct t. exact t. Defined.
 
-Definition rm_void_pair {node root : FinDecType} (pns : type node + type (findec_sum findec_void root)):
+Definition rm_void_pair {node root : FinDecType} (pns : type node + type (findec_sum voidfd root)):
   type node + type root :=
   match pns with 
   | inl n => inl n
@@ -1212,8 +1213,8 @@ Definition rm_void_pair {node root : FinDecType} (pns : type node + type (findec
 
 
 Definition rm_void_parent' {s1 r1 node0: FinDecType} 
-  (p : type node0 + type (findec_sum findec_void s1) ->
-    type node0 + type (findec_sum findec_void r1)) : 
+  (p : type node0 + type (findec_sum voidfd s1) ->
+    type node0 + type (findec_sum voidfd r1)) : 
     type node0 + type s1 ->
       type node0 + type r1 :=
   (fun ns => match ns with 
@@ -1222,7 +1223,7 @@ Definition rm_void_parent' {s1 r1 node0: FinDecType}
     end).   
 
 Definition rm_void_link {i1 o1 node0 edge0: FinDecType} {control0 : (type node0) -> Kappa} 
-  (l : type (findec_sum i1 findec_void) + Port control0 ->
+  (l : type (findec_sum i1 voidfd) + Port control0 ->
     type (findec_sum i1 o1) + type edge0) : 
       type i1 + Port control0 ->
         type (findec_sum i1 o1) + type edge0 :=
@@ -1237,8 +1238,8 @@ Definition rm_void_link {i1 o1 node0 edge0: FinDecType} {control0 : (type node0)
   end end).   
 
 Lemma acyclic_rm_void_parent {node s r: FinDecType} {n:type node}
-  {p: type node + type (findec_sum findec_void s) ->
-  type node + type (findec_sum findec_void r)} :
+  {p: type node + type (findec_sum voidfd s) ->
+  type node + type (findec_sum voidfd r)} :
   Acc (fun n' n : type node => p (inl n) = inl n') n
   -> Acc
   (fun n' n0 : type node => rm_void_parent' p (inl n0) = inl n') n.
@@ -1255,7 +1256,7 @@ Lemma acyclic_rm_void_parent {node s r: FinDecType} {n:type node}
   Admitted.
 
 Definition rm_void_finDecSum {s1 i1 o1 r1: FinDecType} 
-  (b : bigraph (findec_sum findec_void s1) (findec_sum i1 findec_void) (findec_sum findec_void r1) (findec_sum i1 o1)) : 
+  (b : bigraph (findec_sum voidfd s1) (findec_sum i1 voidfd) (findec_sum voidfd r1) (findec_sum i1 o1)) : 
   bigraph s1 i1 r1 (findec_sum i1 o1).
   Proof. 
   destruct b.
@@ -1277,34 +1278,33 @@ Definition rm_void_finDecSum {s1 i1 o1 r1: FinDecType}
 
 
 Definition nest {s1 i1 r1 o1 i2 : FinDecType} 
-  (b1 : bigraph s1 findec_void r1 o1) (b2 : bigraph findec_void i2 s1 i1) :=
-  (rm_void_finDecSum ((@bigraph_identity findec_void i1) || b1)) <<o>> b2.
+  (b1 : bigraph s1 voidfd r1 o1) (b2 : bigraph voidfd i2 s1 i1) :=
+  (rm_void_finDecSum ((@bigraph_identity voidfd i1) || b1)) <<o>> b2.
 
 Definition nest' {I m X n Y : FinDecType} 
-  (F : bigraph findec_void I m X) (G : bigraph m findec_void n Y) 
-  : bigraph findec_void I n (findec_sum X Y) :=
-  (rm_void_finDecSum ((@bigraph_identity findec_void X) || G)) <<o>> F.
+  (F : bigraph voidfd I m X) (G : bigraph m voidfd n Y) 
+  : bigraph voidfd I n (findec_sum X Y) :=
+  (rm_void_finDecSum ((@bigraph_identity voidfd X) || G)) <<o>> F.
 
 Example I : FinDecType. Admitted.
 Example m : FinDecType. Admitted.
 Example X : FinDecType. Admitted.
 Example n : FinDecType. Admitted.
 Example Y : FinDecType. Admitted.
-Example F : bigraph findec_void I m X. Admitted.
-Example G : bigraph m findec_void n Y. Admitted.
+Example F : bigraph voidfd I m X. Admitted.
+Example G : bigraph m voidfd n Y. Admitted.
 
-Check (@bigraph_identity findec_void X) || G.
-Check rm_void_finDecSum ((@bigraph_identity findec_void X) || G).
-Check (rm_void_finDecSum ((@bigraph_identity findec_void X) || G)) <<o>> F.
+Check (@bigraph_identity voidfd X) || G.
+Check rm_void_finDecSum ((@bigraph_identity voidfd X) || G).
+Check (rm_void_finDecSum ((@bigraph_identity voidfd X) || G)) <<o>> F.
 Check nest' F G.
 
-Example b1 {s1 r1 o1}: bigraph s1 findec_void r1 o1. Admitted.
-Example b2 {s1 i2 i1}: bigraph findec_void i2 s1 i1. Admitted.
+Example b1 {s1 r1 o1}: bigraph s1 voidfd r1 o1. Admitted.
+Example b2 {s1 i2 i1}: bigraph voidfd i2 s1 i1. Admitted.
 
 Check nest b1 b2.
 
 End NestingBig.
-
 
 
 
@@ -1355,19 +1355,23 @@ Lemma symmetry_S4 {I J K} :
 
 End Bigraphs.
 
-Module MyBigraphs := Bigraphs.
-Import Bigraphs.
-Definition MyKappa : Type := type (findec_fin 3).
-Example zero : MyKappa. exists 0. auto. Defined.
-Example un : MyKappa. exists 1. auto. Defined.
-Example deux : MyKappa. exists 2. auto. Defined.
 
-Definition MyArity : MyKappa -> nat := (fun 
+Export Bigraphs.
+
+Module MyBigraphs := Bigraphs. (*with (Kappa := type (findec_fin 3)).*)
+Definition Kappa : Type := type (findec_fin 3).
+Example zero : Kappa. exists 0. auto. Defined.
+Example un : Kappa. exists 1. auto. Defined.
+Example deux : Kappa. exists 2. auto. Defined.
+
+Definition MyArity : Kappa -> nat := (fun 
     mk => match mk with 
     | exist _ n pf => n + 1
     end
   ).
-  
+
+Check bigraph.
+Print bigraph.
 Example Kxyz : 
   bigraph (findec_fin 1) (findec_fin 0) (findec_fin 1) (findec_fin 3).
   apply (Big
